Let $X \in \cbrak{0,1}$ where 0 represents tossing a coin.  Let $ Y_i \in \cbrak{3,6,n}$ represent the outcome of a die. $n \ne 3,6$.  Let $Z \in \cbrak{0,1}$ represent a coin toss where 1 represents tail.  Suppose the coin toss happens after $k$ trials of the die.  This means that the outcome of the $k$ trials is either 3 or 6.
{\tiny
\begin{multline}
\pr{Z = 1,Y_k=n,\prod_{i=1}^{k-1}\cbrak{Y_i \ne n}|1-\prod_{i=1}^{k-1}\cbrak{Y_i \ne 3}}
\\
=\frac{\pr{Z = 1,Y_k=n,\prod_{i=1}^{k-1}\cbrak{Y_i \ne n},1-\prod_{i=1}^{k-1}\cbrak{Y_i \ne 3}}}{\pr{1-\prod_{i=1}^{k-1}\cbrak{Y_i \ne 3}}}
\\
=\frac{\pr{Z = 1}\pr{Y_k=n}\pr{\prod_{i=1}^{k-1}\cbrak{Y_i \ne n}\sbrak{1-\prod_{i=1}^{k-1}\cbrak{Y_i \ne 3}}}}{\pr{1-\prod_{i=1}^{k-1}\cbrak{Y_i \ne 3}}}
\\
=\frac{\pr{Z = 1}\pr{Y_k=n}\sbrak{\pr{\prod_{i=1}^{k-1}\cbrak{Y_i \ne n}}-\pr{\prod_{i=1}^{k-1}\cbrak{Y_i \ne n}\cbrak{Y_i \ne 3}}}}{1-\pr{\prod_{i=1}^{k-1}\cbrak{Y_i \ne 3}}}
\\
=\frac{\pr{Z = 1}\pr{Y_k=n}\sbrak{\pr{\prod_{i=1}^{k-1}\cbrak{Y_i \ne n}}-\pr{\prod_{i=1}^{k-1}\cbrak{Y_i =6 }}}}{1-\pr{\prod_{i=1}^{k-1}\cbrak{Y_i \ne 3}}}
\\
=\frac{\frac{1}{2}\times \frac{4}{6}\sbrak{\brak{\frac{2}{6}}^{k-1}-\brak{\frac{1}{6}}^{k-1}}}{1-\brak{\frac{5}{6}}^{k-1}}
= \frac{2^{k-1}-1}{3\brak{6^{k-1}-5^{k-1}}}
\end{multline}
}

